\begin{table}[b]
	\centering
	%\caption{Hodge-Duale}
	%\label{maxwell:section:teil1:Hodge-Tabelle}
	\begin{tabularx}{\textwidth}{ 
			| >{\centering\arraybackslash}X 
			| >{\centering\arraybackslash}X 
			| >{\centering\arraybackslash}X | }
		\hline
		\textbf{1-Form} & \textbf{2-Form} & \textbf{3-Form} \\
		\hline
		\( \rule{0pt}{1.5em} {\ast} dx^0 = -dx^1 \wedge dx^2 \wedge dx^3 \) \newline
	\( {\ast} dx^1 = -dx^0 \wedge dx^2 \wedge dx^3 \) \newline
	\( {\ast} dx^2 = \phantom{-} dx^0 \wedge dx^1 \wedge dx^3 \) \newline
	\( {\ast} dx^3 = -dx^0 \wedge dx^1 \wedge dx^2 \, \) 
	&
	\( \rule{0pt}{1.5em} {\ast} (dx^0 \wedge dx^1) = -dx^2 \wedge dx^3 \) \newline
	\( {\ast} (dx^1 \wedge dx^2) = \phantom{-} dx^0 \wedge dx^3 \) \newline
	\( {\ast} (dx^2 \wedge dx^3) = \phantom{-} dx^0 \wedge dx^1 \) \newline
	\( {\ast} (dx^0 \wedge dx^2) = \phantom{-} dx^1 \wedge dx^3 \) \newline
	\( {\ast} (dx^0 \wedge dx^3) = -dx^1 \wedge dx^2 \) \newline
	\( {\ast} (dx^1 \wedge dx^3) = -dx^0 \wedge dx^2 \)
	&
	\( \rule{0pt}{1.5em} {\ast} (dx^0 \wedge dx^1 \wedge dx^2) = -dx^3 \) \newline
	\( {\ast} (dx^0 \wedge dx^1 \wedge dx^3) = \phantom{-} dx^2 \) \newline
	\( {\ast} (dx^0 \wedge dx^2 \wedge dx^3) = -dx^1 \) \newline
	\( {\ast} (dx^1 \wedge dx^2 \wedge dx^3) = -dx^0 \)
		\\
		\hline
	\end{tabularx}
	\caption{Tabelle aller Hodge-Duale von 1-, 2-, und 3-Formen mit $({-}{+}{+}{+})$-Signatur}
	\label{maxwell:section:teil1:Hodge-Tabelle}
\end{table}
